<?xml version="1.0" encoding="utf-8" ?>

<!DOCTYPE rdf:RDF [
    <!ENTITY rdf "http://www.w3.org/1999/02/22-rdf-syntax-ns#" >
    <!ENTITY rdfs "http://www.w3.org/2000/01/rdf-schema#" >
    <!ENTITY xsd "http://www.w3.org/2001/XMLSchema#" >
    <!ENTITY owl "http://www.w3.org/2002/07/owl#" >
    <!ENTITY dcterms "http://purl.org/dc/terms/" >
    <!ENTITY foaf "http://xmlns.com/foaf/0.1/" >
    <!ENTITY cc "http://creativecommons.org/ns#" >
    <!ENTITY vann "http://purl.org/vocab/vann/" >
]>

<rdf:RDF
    xmlns="http://cabas.ugr.es/ontology/ugr#"
    xmlns:rdf="&rdf;"
    xmlns:rdfs="&rdfs;"
    xmlns:xsd="&xsd;"
    xmlns:owl="&owl;"
    xmlns:dcterms="&dcterms;"
    xmlns:foaf="&foaf;"
    xmlns:cc="&cc;"
    xmlns:vann="&vann;">

    <owl:Ontology rdf:about="http://cabas.ugr.es/ontology/ugr#">
        <rdfs:label xml:lang="es">Ontología de la Universidad de Granada</rdfs:label>
        <rdfs:label xml:lang="en">Ontology of the University of Granada</rdfs:label>
        <rdfs:comment xml:lang="es">
            Ontología creada para describir los conjuntos de datos abiertos de la Universidad de Granada.
        </rdfs:comment>
        <rdfs:comment xml:lang="en">
            Ontology created to describe the open data sets of the University of Granada.
        </rdfs:comment>
        <dcterms:title xml:lang="es">Ontología de la Universidad de Granada</dcterms:title>
        <dcterms:title xml:lang="en">Ontology of the University of Granada</dcterms:title>
        <dcterms:description xml:lang="es">
            La ontología de la Universidad de Granada define las clases y propiedades utilizadas en los conjuntos de datos abiertos de la propia Universidad.
        </dcterms:description>
        <dcterms:description xml:lang="en">
            The ontology of the University of Granada defines the classes and properties used in the open data sets of the University itself.
        </dcterms:description>
        <owl:versionInfo xml:lang="es">1.0</owl:versionInfo>
        <dcterms:created rdf:datatype="&xsd;date">2017-06-18</dcterms:created>
        <vann:preferredNamespacePrefix>ugr</vann:preferredNamespacePrefix>
        <vann:preferredNamespaceUri>http://cabas.ugr.es/ontology/ugr#</vann:preferredNamespaceUri>
        <foaf:homepage rdf:resource="http://opendata.ugr.es" />
        <dcterms:source rdf:resource="http://opendata.ugr.es" />
        <dcterms:creator>Germán Martínez Maldonado</dcterms:creator>
        <foaf:maker rdf:resource="https://github.com/germaaan" />
        <dcterms:publisher>Oficina de Software Libre de la Universidad de Granada</dcterms:publisher>
        <cc:license rdf:resource="http://www.gnu.org/copyleft/fdl.html" />
        <cc:license rdf:resource="http://creativecommons.org/licenses/by-sa/4.0/" />
    </owl:Ontology>

    <!--
    ///////////////////////////////////////////////////////////////////////////////////////
    //
    // Classes
    //
    ///////////////////////////////////////////////////////////////////////////////////////
     -->

     <owl:Class rdf:about="#RamaConocimiento">
         <rdfs:label xml:lang="es">Rama de conocimiento</rdfs:label>
         <rdfs:label xml:lang="en">Branch of knowledge</rdfs:label>
         <rdfs:comment xml:lang="es">Una rama de conocimiento es el campo en el que se agrupan diferentes titulaciones con un conjunto de materias similares lo que hace que tengan una identidad semejante.</rdfs:comment>
         <rdfs:comment xml:lang="en">A branch of knowledge is the field in which different degrees are grouped with a set of similar subjects which makes them have a similar identity.</rdfs:comment>
     </owl:Class>

    <owl:Class rdf:about="#Titulación">
        <rdfs:subClassOf rdf:resource="#RamaConocimiento"/>
        <rdfs:label xml:lang="es">Titulación</rdfs:label>
        <rdfs:label xml:lang="en">Degree</rdfs:label>
        <rdfs:comment xml:lang="es">Una titulación es el reconocimiento que se obtiene después de superar los estudios universitarios de grado o máster; reconocíendo una formación general, en una o varias disciplinas, orientada a la preparación para el
            desempeño de actividades de carácter profesional.</rdfs:comment>
        <rdfs:comment xml:lang="en">A degree is the recognition that is obtained after overcoming university studies of degree or masters; Recognizing a general formation, in one or several disciplines, oriented to the preparation for the performance of professional activities.</rdfs:comment>
    </owl:Class>

    <owl:Class rdf:about="#Persona">
        <rdfs:label xml:lang="es">Persona</rdfs:label>
        <rdfs:label xml:lang="en">Person</rdfs:label>
        <rdfs:comment xml:lang="es">Una persona es un ser racional e inteligente, consciente de sí mismo y de sus actos que cuenta con identidad propia.</rdfs:comment>
        <rdfs:comment xml:lang="en">A person is a rational and intelligent being, aware of himself and his acts that has its own identity.</rdfs:comment>
        <owl:equivalentClass rdf:resource="http://dbpedia.org/ontology/Person" />
        <owl:equivalentClass rdf:resource="https://www.wikidata.org/wiki/Q215627" />
    </owl:Class>

    <owl:Class rdf:about="#Hombres">
        <rdfs:subClassOf rdf:resource="#Persona"/>
        <rdfs:label xml:lang="es">Hombres</rdfs:label>
        <rdfs:label xml:lang="en">Men</rdfs:label>
        <rdfs:comment xml:lang="es">Número de estudiantes hombres.</rdfs:comment>
        <rdfs:comment xml:lang="en">Number of male students.</rdfs:comment>
        <owl:equivalentClass rdf:resource="http://schema.org/Male" />
        <owl:equivalentClass rdf:resource="https://www.wikidata.org/wiki/Q6581097" />
    </owl:Class>

    <owl:Class rdf:about="#Mujeres">
        <rdfs:subClassOf rdf:resource="#Persona"/>
        <rdfs:label xml:lang="es">Mujeres</rdfs:label>
        <rdfs:label xml:lang="en">Women</rdfs:label>
        <rdfs:comment xml:lang="es">Número de estudiantes mujeres.</rdfs:comment>
        <rdfs:comment xml:lang="en">Number of female students.</rdfs:comment>
        <owl:equivalentClass rdf:resource="http://schema.org/Female" />
        <owl:equivalentClass rdf:resource="https://www.wikidata.org/wiki/Q6581072" />
    </owl:Class>

    <!--
    ///////////////////////////////////////////////////////////////////////////////////////
    //
    // Object Properties
    //
    ///////////////////////////////////////////////////////////////////////////////////////
     -->

    <owl:ObjectProperty rdf:about="#tieneRamaConocimiento">
        <rdf:type rdf:resource="&owl;FunctionalProperty" />
        <rdf:type rdf:resource="&rdf;Property" />
        <rdfs:label xml:lang="es">tiene rama de conocimiento</rdfs:label>
        <rdfs:label xml:lang="en">has branch of knowledge</rdfs:label>
        <rdfs:comment xml:lang="es">Una titulación pertenece a una rama de conocimiento.</rdfs:comment>
        <rdfs:comment xml:lang="en">A degree belongs to a branch of knowledge.</rdfs:comment>
        <rdfs:domain rdf:resource="#Titulación" />
        <rdfs:range rdf:resource="#RamaConocimiento" />
        <owl:sameAs rdf:resource="#tieneRamaConocimiento" />
        <owl:inverseOf rdf:resource="#tieneTitulación" />
    </owl:ObjectProperty>

    <owl:ObjectProperty rdf:about="#tieneTitulación">
        <rdf:type rdf:resource="&rdf;Property" />
        <rdfs:label xml:lang="es">tiene titulación</rdfs:label>
        <rdfs:label xml:lang="en">has degree</rdfs:label>
        <rdfs:comment xml:lang="es">Una rama de conocimiento engloba diferentes titulaciones.</rdfs:comment>
        <rdfs:comment xml:lang="en">A branch of knowledge encompasses different degrees.</rdfs:comment>
        <rdfs:domain rdf:resource="#RamaConocimiento" />
        <rdfs:range rdf:resource="#Titulación" />
        <owl:sameAs rdf:resource="#tieneTitulacion" />
        <owl:inverseOf rdf:resource="#tieneRamaConocimiento" />
    </owl:ObjectProperty>

    <!--
    ///////////////////////////////////////////////////////////////////////////////////////
    //
    // Datatype properties
    //
    ///////////////////////////////////////////////////////////////////////////////////////
     -->



    <!--
    ///////////////////////////////////////////////////////////////////////////////////////
    //
    // General axioms
    //
    ///////////////////////////////////////////////////////////////////////////////////////
     -->

    <owl:AllDisjointProperties>
        <owl:members rdf:parseType="Collection">
            <rdf:Description rdf:about="#tieneRamaConocimiento" />
            <rdf:Description rdf:about="#tieneTitulacion" />
        </owl:members>
    </owl:AllDisjointProperties>

    <owl:AllDisjointClasses>
        <owl:members rdf:parseType="Collection">
            <rdf:Description rdf:about="#Hombres" />
            <rdf:Description rdf:about="#Mujeres" />
        </owl:members>
    </owl:AllDisjointClasses>

    <owl:AllDisjointClasses>
        <owl:members rdf:parseType="Collection">
            <rdf:Description rdf:about="#Titulación" />
            <rdf:Description rdf:about="#RamaConocimiento" />
        </owl:members>
    </owl:AllDisjointClasses>
</rdf:RDF>
