<?xml version="1.0" encoding="utf-8" ?>

<!DOCTYPE rdf:RDF [
    <!ENTITY rdf "http://www.w3.org/1999/02/22-rdf-syntax-ns#" >
    <!ENTITY rdfs "http://www.w3.org/2000/01/rdf-schema#" >
    <!ENTITY owl "http://www.w3.org/2002/07/owl#" >
    <!ENTITY dct "http://purl.org/dc/terms/" >
    <!ENTITY ns4 "http://creativecommons.org/ns#" >
    <!ENTITY ns5 "http://purl.org/vocab/vann/" >
    <!ENTITY foaf "http://xmlns.com/foaf/0.1/" >
]>

<rdf:RDF
    xmlns:rdf="http://www.w3.org/1999/02/22-rdf-syntax-ns#"
    xmlns:rdfs="http://www.w3.org/2000/01/rdf-schema#"
    xmlns:dct="http://purl.org/dc/terms/"
    xmlns:owl="http://www.w3.org/2002/07/owl#"
    xmlns:ns4="http://creativecommons.org/ns#"
    xmlns:ns5="http://purl.org/vocab/vann/"
    xmlns:foaf="http://xmlns.com/foaf/0.1/">

    <rdf:Description rdf:about="http://cabas.ugr.es/ontology/ugr#">
        <rdf:type rdf:resource="http://www.w3.org/2002/07/owl#Ontology"/>
        <rdf:type rdf:resource="http://purl.org/vocommons/voaf#Vocabulary"/>
        <dct:modified>2017-06-18T13:05Z</dct:modified>
        <rdfs:comment xml:lang="es">
            Ontología creada para describir los conjuntos de datos abiertos de la Universidad de Granada.
        </rdfs:comment>
        <rdfs:comment xml:lang="en">
            Ontology created to describe the open data sets of the University of Granada.
        </rdfs:comment>
        <owl:versionInfo xml:lang="es">1.0</owl:versionInfo>
        <owl:sameAs rdf:resource="http://cabas.ugr.es/ontology/ugr#"/>
        <ns4:license rdf:resource="http://www.gnu.org/copyleft/fdl.html"/>
        <ns4:license rdf:resource="http://creativecommons.org/licenses/by-sa/4.0/"/>
        <dct:issued>2016-09-07T12:00Z</dct:issued>
        <ns5:preferredNamespacePrefix>ugr</ns5:preferredNamespacePrefix>
        <ns5:preferredNamespaceUri>http://cabas.ugr.es/ontology/ugr#</ns5:preferredNamespaceUri>
        <foaf:homepage rdf:resource="http://opendata.ugr.es"/>
        <dct:title xml:lang="es">Ontología de la Universidad de Granada</dct:title>
        <dct:title xml:lang="en">Ontology of the University of Granada</dct:title>
        <dct:description xml:lang="es">
            La ontología de la Universidad de Granada define las clases y propiedades utilizadas en los conjuntos de datos abiertos de la propia Universidad.
        </dct:description>
        <dct:description xml:lang="en">
            The ontology of the University of Granada defines the classes and properties used in the open data sets of the University itself.
        </dct:description>
        <dct:creator>Germán Martínez Maldonado</dct:creator>
        <dct:source rdf:resource="http://opendata.ugr.es"/>
        <dct:publisher>Oficina de Software Libre de la Universidad de Granada</dct:publisher>
    </rdf:Description>

    <!--
    ///////////////////////////////////////////////////////////////////////////////////////
    //
    // Object Properties
    //
    ///////////////////////////////////////////////////////////////////////////////////////
     -->

    <rdf:Description rdf:about="http://cabas.ugr.es/ontology/ugr#tieneRamaConocimiento">
        <rdf:type rdf:resource="http://www.w3.org/2002/07/owl#ObjectProperty"/>
        <rdf:type rdf:resource="http://www.w3.org/1999/02/22-rdf-syntax-ns#Property"/>
        <rdfs:label xml:lang="es">tiene rama de conocimiento</rdfs:label>
        <rdfs:label xml:lang="en">has branch of knowledge</rdfs:label>
        <rdfs:comment xml:lang="es">Una titulación pertenece a una rama de conocimiento.</rdfs:comment>
        <rdfs:comment xml:lang="en">A degree belongs to a branch of knowledge.</rdfs:comment>
        <rdfs:domain rdf:resource="http://cabas.ugr.es/ontology/ugr#Titulación"/>
        <rdfs:range rdf:resource="http://cabas.ugr.es/ontology/ugr#RamaConocimiento"/>
        <owl:sameAs rdf:resource="http://cabas.ugr.es/ontology/ugr#tieneRamaConocimiento"/>
        <owl:inverseOf rdf:resource="http://cabas.ugr.es/ontology/ugr#tieneTitulación"/>
    </rdf:Description>

    <rdf:Description rdf:about="http://cabas.ugr.es/ontology/ugr#tieneTitulación">
        <rdf:type rdf:resource="http://www.w3.org/2002/07/owl#ObjectProperty"/>
        <rdf:type rdf:resource="http://www.w3.org/1999/02/22-rdf-syntax-ns#Property"/>
        <rdfs:label xml:lang="es">tiene titulación</rdfs:label>
        <rdfs:label xml:lang="en">has degree</rdfs:label>
        <rdfs:comment xml:lang="es">Una rama de conocimiento engloba diferentes titulaciones.</rdfs:comment>
        <rdfs:comment xml:lang="en">A branch of knowledge encompasses different degrees.</rdfs:comment>
        <rdfs:domain rdf:resource="http://cabas.ugr.es/ontology/ugr#RamaConocimiento"/>
        <rdfs:range rdf:resource="http://cabas.ugr.es/ontology/ugr#Titulación"/>
        <owl:sameAs rdf:resource="http://cabas.ugr.es/ontology/ugr#tieneTitulacion"/>
        <owl:inverseOf rdf:resource="http://cabas.ugr.es/ontology/ugr#tieneRamaConocimiento"/>
    </rdf:Description>

    <!--
    ///////////////////////////////////////////////////////////////////////////////////////
    //
    // Data properties
    //
    ///////////////////////////////////////////////////////////////////////////////////////
     -->

    <rdf:Description rdf:about="http://cabas.ugr.es/ontology/ugr#hombres">
        <rdf:type rdf:resource="http://www.w3.org/2002/07/owl#DatatypeProperty"/>
        <rdf:type rdf:resource="http://www.w3.org/1999/02/22-rdf-syntax-ns#Property"/>
        <rdfs:label xml:lang="es">hombres</rdfs:label>
        <rdfs:label xml:lang="en">men</rdfs:label>
        <rdfs:comment xml:lang="es">Número de estudiantes hombres.</rdfs:comment>
        <rdfs:comment xml:lang="en">Number of male students.</rdfs:comment>
        <rdfs:domain rdf:resource="http://cabas.ugr.es/resources/MatriculasGrado1516"/>
        <rdfs:range rdf:datatype="http://www.w3.org/2001/XMLSchema#integer"/>
        <owl:sameAs rdf:resource="http://cabas.ugr.es/ontology/ugr#hombres"/>
        <owl:equivalentProperty rdf:resource="https://schema.org/Male"/>
        <owl:inverseOf rdf:resource="http://cabas.ugr.es/ontology/ugr#mujeres"/>
    </rdf:Description>

    <rdf:Description rdf:about="http://cabas.ugr.es/ontology/ugr#mujeres">
        <rdf:type rdf:resource="http://www.w3.org/2002/07/owl#DatatypeProperty"/>
        <rdf:type rdf:resource="http://www.w3.org/1999/02/22-rdf-syntax-ns#Property"/>
        <rdfs:label xml:lang="es">mujeres</rdfs:label>
        <rdfs:label xml:lang="en">women</rdfs:label>
        <rdfs:comment xml:lang="es">Número de estudiantes mujeres.</rdfs:comment>
        <rdfs:comment xml:lang="en">Number of female students.</rdfs:comment>
        <rdfs:domain rdf:resource="http://cabas.ugr.es/resources/MatriculasGrado1516"/>
        <rdfs:range rdf:datatype="http://www.w3.org/2001/XMLSchema#integer"/>
        <owl:sameAs rdf:resource="http://cabas.ugr.es/ontology/ugr#mujeres"/>
        <owl:equivalentProperty rdf:resource="https://schema.org/Female"/>
        <owl:inverseOf rdf:resource="http://cabas.ugr.es/ontology/ugr#hombres"/>
    </rdf:Description>

    <!--
    ///////////////////////////////////////////////////////////////////////////////////////
    //
    // Classes
    //
    ///////////////////////////////////////////////////////////////////////////////////////
     -->

    <rdf:Description rdf:about="http://cabas.ugr.es/ontology/ugr#Titulación">
        <rdf:type rdf:resource="http://www.w3.org/2002/07/owl#Class"/>
        <rdf:type rdf:resource="http://www.w3.org/1999/02/22-rdf-syntax-ns#Class"/>
        <rdfs:label xml:lang="es">titulación</rdfs:label>
        <rdfs:label xml:lang="en">degree</rdfs:label>
        <rdfs:comment xml:lang="es">Una titulación es el reconocimiento que se obtiene después de superar los estudios universitarios de grado o máster; reconocíendo una formación general, en una o varias disciplinas, orientada a la preparación para el
            desempeño de actividades de carácter profesional.</rdfs:comment>
        <rdfs:comment xml:lang="en">A degree is the recognition that is obtained after overcoming university studies of degree or masters; Recognizing a general formation, in one or several disciplines, oriented to the preparation for the performance of professional activities.</rdfs:comment>
        <owl:sameAs rdf:resource="http://cabas.ugr.es/ontology/ugr#Titulación"/>
        <owl:equivalentClass rdf:resource="http://vivoweb.org/ontology/core#AcademicDegree"/>
    </rdf:Description>

    <rdf:Description rdf:about="http://cabas.ugr.es/ontology/ugr#RamaConocimiento">
        <rdf:type rdf:resource="http://www.w3.org/2002/07/owl#Class"/>
        <rdf:type rdf:resource="http://www.w3.org/1999/02/22-rdf-syntax-ns#Class"/>
        <rdfs:label xml:lang="en">branch of knowledge</rdfs:label>
        <rdfs:label xml:lang="es">rama de conocimiento</rdfs:label>
        <rdfs:comment xml:lang="es">Una rama de conocimiento es el campo en el que se agrupan diferentes titulaciones con un conjunto de materias similares lo que hace que tengan una identidad semejante.</rdfs:comment>
        <rdfs:comment xml:lang="en">A branch of knowledge is the field in which different degrees are grouped with a set of similar subjects which makes them have a similar identity.</rdfs:comment>
        <owl:sameAs rdf:resource="http://cabas.ugr.es/ontology/ugr#RamaConocimiento"/>
    </rdf:Description>

    <!--
    ///////////////////////////////////////////////////////////////////////////////////////
    //
    // General axioms
    //
    ///////////////////////////////////////////////////////////////////////////////////////
     -->

    <rdf:Description>
        <rdf:type rdf:resource="https://www.w3.org/2002/07/owl#AllDisjointProperties"/>
        <owl:members rdf:parseType="Collection">
            <rdf:Description rdf:about="http://cabas.ugr.es/ontology/ugr#tieneRamaConocimiento"/>
            <rdf:Description rdf:about="http://cabas.ugr.es/ontology/ugr#tieneTitulacion"/>
        </owl:members>
    </rdf:Description>
    <rdf:Description>
        <rdf:type rdf:resource="https://www.w3.org/2002/07/owl#AllDisjointProperties"/>
        <owl:members rdf:parseType="Collection">
            <rdf:Description rdf:about="http://cabas.ugr.es/ontology/ugr#hombres"/>
            <rdf:Description rdf:about="http://cabas.ugr.es/ontology/ugr#mujeres"/>
        </owl:members>
    </rdf:Description>
    <rdf:Description>
        <rdf:type rdf:resource="https://www.w3.org/2002/07/owl#AllDisjointClasses"/>
        <owl:members rdf:parseType="Collection">
            <rdf:Description rdf:about="http://cabas.ugr.es/ontology/ugr#Titulación"/>
            <rdf:Description rdf:about="http://cabas.ugr.es/ontology/ugr#RamaConocimiento"/>
        </owl:members>
    </rdf:Description>
</rdf:RDF>
